fixed reordere

Reorderer/Impl.v
@@ -5,110 +5,125 @@ Section Reorderer.
   Context `{ReordererParams}.
   Class ReordererImplParams :=
     {
-      (* Methods for interacting with the response buffer (holding Maybe
-     Insts). *)
+      (* Methods for interacting with the response buffer (holding Maybe Insts). *)
+      rfName: string;
       rfRead: string;
       rfWrite: string;
       (* methods for interacting with the address memory, which keeps
-     track of the address each request corresponds to *)
+         track of the address each request corresponds to *)
+      arfName: string;
       arfRead: string;
       arfWrite: string;
-      handlingName: string;
-      givingName: string;
+
+      enqPtr: string;
+      deqPtr: string;
     }.
 
   Section withParams.
     Context `{ReordererImplParams}.
     Local Open Scope kami_expr.
     Local Open Scope kami_action.
+
+    Definition reqIdLen := Nat.pow 2 reqIdSz.
     
     Section withTy.
 
-    (* Conceptual rule *)
-   Definition handle
-     (prefetcherCallback: forall {ty}, ty ReordererRes -> ActionT ty Void)
-     ty
-     : ActionT ty Void
-     := Read handling: ReordererReqId <- handlingName;
-        Call MRes: Maybe MInst <- rfRead(#handling: ReordererReqId);
-        (* Call req: ReordererReq <- arfRead(#handling: ReordererReqId); *)
-        Call vaddr: VAddr <- arfRead(#handling: ReordererReqId);
-        LET resp
-          :  ReordererRes
-          <- STRUCT {
-               "vaddr" ::= #vaddr;
-               "inst"  ::= #MRes @% "data"
-             };
-        If #MRes @% "valid"
-          then
-            LETA _ <- prefetcherCallback (resp : ty ReordererRes);
-            Write handlingName <- #handling + $1;
-            Retv;
+      (* Conceptual rule *)
+      Definition responseToPrefetcher
+                 (prefetcherCallback: forall {ty}, ty ReordererRes -> ActionT ty Void)
+                 ty
+      : ActionT ty Void
+        := Read deqPFull: ReordererPtr <- deqPtr;
+           Read enqPFull: ReordererPtr <- enqPtr;
+           LET deqP: ReordererReqId <- UniBit (TruncLsb _ 1) #deqPFull;
+           Call inst: Maybe MInst <- rfRead(#deqP: ReordererReqId);
+           Call vaddr: VAddr <- arfRead(#deqP: ReordererReqId);
+           LET resp
+           :  ReordererRes
+                <- STRUCT {
+                  "vaddr" ::= #vaddr;
+                  "inst"  ::= #inst @% "data"
+                };
+           If (#deqPFull != #enqPFull) && #inst @% "valid"
+           then
+             LETA _ <- prefetcherCallback (resp : ty ReordererRes);
+             Write deqPtr <- #deqPFull + $1;
+             Retv;
+           Retv.
+
+      (* Action the arbiter will call when giving us (the reorderer) the
+         response to a prior request *)
+      Definition reordererCallback ty (resp: ty ReordererArbiterRes): ActionT ty Void :=
+        LET idx: ReordererReqId <- #resp @% "tag";
+        LET res: MInst <- #resp @% "resp";
+        Call rfWrite(STRUCT { "addr" ::= #idx;
+                              "data" ::= Valid #res } : WriteRq reqIdSz (Maybe MInst));
         Retv.
 
-   (* Action the arbiter will call when giving us (the reorderer) the
-      response to a prior request *)
-   Definition reordererCallback ty (resp: ty ReordererArbiterRes): ActionT ty Void :=
-    LET idx: ReordererReqId <- #resp @% "tag";
-    LET res: MInst <- #resp @% "resp";
-    Call rfWrite(STRUCT { "addr" ::= #idx;
-                          "data" ::= Valid #res } : WriteRq reqIdSz (Maybe MInst));
-    Retv.
-
-   (* TODO: Completely broken. *)
-   (* Action the prefetcher will ultimately use to make an order-preserving request for instructions at some address *)
-   Definition sendReq
-     ty
-     (memReq
-       : ty ReordererArbiterReq ->
-         ActionT ty ReordererArbiterImmRes)
-      (req: ty ReordererReq)
-     :  ActionT ty ReordererImmRes
-     := Read giving: ReordererReqId <- givingName;
-        Read handling: ReordererReqId <- handlingName;
-        LET arbiterReq
-          :  ReordererArbiterReq
-          <- STRUCT {
-               "tag" ::= #giving;
-               "req" ::= #req @% "paddr"
-             };
-        If (#giving + $1) != #handling
-          then (* we can give a new reqid without forgetting the next one to service *)
-            LETA res <- memReq arbiterReq;
-            If #res @% "ready"
-              then
-                Write givingName: ReordererReqId <- #giving + $1;
-                Call rfWrite(STRUCT { "addr" ::= #giving;
-                                      "data" ::= Invalid } : WriteRq reqIdSz (Maybe MInst));
-                Call arfWrite
-                  (STRUCT {
-                     "addr" ::= #giving;
-                     "data" ::= #req @% "vaddr"
-                   } : WriteRq reqIdSz VAddr);
-                Retv;
-           Ret #res
-         else
-           Ret (STRUCT {
-             "ready" ::= $$false;
-             "info"  ::= $$(getDefaultConst ImmRes)
-           } : ReordererImmRes @# ty)
-         as ret;
-         Ret #ret.
-   End withTy.
+      Definition sendReq
+                 ty
+                 (memReq
+                  : ty ReordererArbiterReq ->
+                    ActionT ty ReordererImmRes)
+                 (req: ty ReordererReq)
+        :  ActionT ty ReordererImmRes
+        := Read enqPFull: ReordererPtr <- enqPtr;
+           Read deqPFull: ReordererPtr <- deqPtr;
+           LET enqP: ReordererReqId <- UniBit (TruncLsb _ 1) #enqPFull;
+           LET deqP: ReordererReqId <- UniBit (TruncLsb _ 1) #deqPFull;
+           LET arbiterReq
+           :  ReordererArbiterReq
+                <- STRUCT {
+                  "tag" ::= #enqP;
+                  "req" ::= #req @% "paddr"
+                };
+           If (#deqPFull + $(Nat.pow 2 reqIdSz)) != #enqPFull
+           then (* we can give a new reqid without forgetting the next one to service *)
+             LETA res <- memReq arbiterReq;
+             If #res @% "ready"
+               then
+                 Write enqPtr <- #enqPFull + $1;
+                 Call rfWrite(STRUCT { "addr" ::= #enqP;
+                                       "data" ::= Invalid } : WriteRq reqIdSz (Maybe MInst));
+                 Call arfWrite
+                   (STRUCT {
+                      "addr" ::= #enqP;
+                      "data" ::= #req @% "vaddr"
+                    } : WriteRq reqIdSz VAddr);
+                 Retv;
+             Ret #res
+           else
+             Ret (STRUCT {
+               "ready" ::= $$false;
+               "info"  ::= $$(getDefaultConst ImmRes)
+             } : ReordererImmRes @# ty)
+           as ret;
+           Ret #ret.
+    End withTy.
 
     Open Scope kami_scope.
     Open Scope kami_expr_scope.
     
-    Definition regs: list RegInitT := makeModule_regs ( Register handlingName: ReordererReqId <- $ 0 ++
-                                                        Register givingName: ReordererReqId <- $ 0 ).
+    Definition regs: list RegInitT := makeModule_regs ( Register enqPtr: ReordererPtr <- $ 0 ++
+                                                        Register deqPtr: ReordererPtr <- $ 0 ).
+
+    Definition regFiles: list RegFileBase :=
+      [ 
+        @Build_RegFileBase false 1 rfName
+                           (Async [rfRead]) rfWrite reqIdSz (Maybe MInst) (@RFNonFile _ _ None);
+          
+        @Build_RegFileBase false 1 arfName
+                           (Async [arfRead]) arfWrite reqIdSz VAddr (@RFNonFile _ _ None)
+      ].
     
-   Instance implReorderer: Reorderer :=
-     {|
-       Reorderer.Ifc.regs := regs;
-       Reorderer.Ifc.regFiles := []; (* TODO: LLEE *)
-       Reorderer.Ifc.handle := handle;
-       Reorderer.Ifc.reordererCallback := reordererCallback;
-       Reorderer.Ifc.sendReq := sendReq
-     |}.
+
+    Instance implReorderer: Reorderer :=
+      {|
+        Reorderer.Ifc.regs := regs;
+        Reorderer.Ifc.regFiles := regFiles;
+        Reorderer.Ifc.responseToPrefetcher := responseToPrefetcher;
+        Reorderer.Ifc.callback := reordererCallback;
+        Reorderer.Ifc.sendReq := sendReq
+      |}.
   End withParams.
 End Reorderer.
